Proved a less trivial example using Send and Receive commands, added new rules to the cstep inductive relation

dist_imp.v
@@ -164,6 +164,8 @@ Inductive cstep : (com * State) -> (com * State) -> Prop :=
   | CS_Ass : forall (sb1 : sb) (rb1 : rb) (st1 : st) (i : id) (n : nat),
       cstep (i ::= (ANum n), state sb1 rb1 st1) 
       (SKIP, state sb1 rb1 (t_update st1 i n))
+  | CS_SeqSkip : forall (c2 : com) (st : State),
+      cstep (SKIP ;; c2, st) (c2, st)
   | CS_SeqStep : forall (st: State) (c1 c1': com) (st' : State) (c2 : com),
       cstep (c1, st) (c1', st') ->
       cstep (c1 ;; c2, st) (c1' ;; c2, st')
@@ -185,21 +187,39 @@ Inductive cstep : (com * State) -> (com * State) -> Prop :=
       ((IFB b THEN (c1;; (WHILE b DO c1 END)) ELSE SKIP FI), state sb1 rb1 st1)
 
   | CS_Send1 : forall (sb1 : sb) (rb1 : rb)
+                      (st1 : st) (a a' : aexp) (x z : id) (c2 : com),
+      a / state sb1 rb1 st1 ==>a a' -> 
+      cstep ((SEND a TO x CALLED z) ;; c2, state sb1 rb1 st1) 
+            ((SEND a' TO x CALLED z) ;; c2, state sb1 rb1 st1)
+  | CS_Send2 : forall (sb1 : sb) (rb1 : rb) (st1 : st) 
+                      (a : aexp) (x z : id) (n : nat) (c2 : com),
+      a = ANum n ->
+      cstep ((SEND a TO x CALLED z) ;; c2, state sb1 rb1 st1) 
+            (SKIP ;; c2, state (app sb1 (cons (a, x, z) nil)) rb1 st1)
+  | CS_Send3 : forall (sb1 : sb) (rb1 : rb)
                       (st1 : st) (a a' : aexp) (x z : id),
       a / state sb1 rb1 st1 ==>a a' -> 
       cstep (SEND a TO x CALLED z, state sb1 rb1 st1) 
             (SEND a' TO x CALLED z, state sb1 rb1 st1)
-  | CS_Send2 : forall (sb1 : sb) (rb1 : rb) (st1 : st) 
+  | CS_Send4 : forall (sb1 : sb) (rb1 : rb) (st1 : st) 
                       (a : aexp) (x z : id) (n : nat),
       a = ANum n ->
       cstep (SEND a TO x CALLED z, state sb1 rb1 st1) 
             (SKIP, state (app sb1 (cons (a, x, z) nil)) rb1 st1)
-  | CS_Rec1 : forall (sb1 : sb) (st1 : st),
-      cstep (RECEIVE, state sb1 nil st1) (SKIP ;; RECEIVE, state sb1 nil st1)
+  | CS_Rec1 : forall (sb1 : sb) (st1 : st) (c2 : com),
+      cstep (RECEIVE ;; c2, state sb1 nil st1) 
+            (SKIP ;; RECEIVE ;; c2, state sb1 nil st1)
   | CS_Rec2 : forall (sb1 : sb) (rb1 : rb) 
-                     (st1 : st) (a : aexp) (x z : id) (c1 : com),
+                     (st1 : st) (a : aexp) (z : id) (c1 : com),
       cstep (RECEIVE ;; c1, state sb1 (app (cons (a, z) nil) rb1) st1) 
-            (x ::= a ;; c1, state sb1 rb1 st1).
+            (z ::= a ;; c1, state sb1 rb1 st1)
+  | CS_Rec3 : forall (sb1 : sb) (st1 : st),
+      cstep (RECEIVE, state sb1 nil st1) 
+            (SKIP ;; RECEIVE, state sb1 nil st1)
+  | CS_Rec4 : forall (sb1 : sb) (rb1 : rb) 
+                     (st1 : st) (a : aexp) (z : id),
+      cstep (RECEIVE, state sb1 (app (cons (a, z) nil) rb1) st1) 
+            (z ::= a, state sb1 rb1 st1).
 
 Inductive imp : Type :=
   | machine : id -> com -> State -> imp.
@@ -218,29 +238,58 @@ Inductive dist_imp : (imp * imp) -> (imp * imp) -> Prop :=
     dist_imp ((machine x c1 (state (cons (a, y, z) sb1) rb1 st1)),
              (machine y c2 (state sb2 rb2 st2)))
             ((machine x c1 (state sb1 rb1 st1)),
-            ((machine y (RECEIVE ;; c2) 
-                (state sb2 (app (cons (a, z) nil) rb2) st2))))
+            ((machine y c2 (state sb2 (app (cons (a, z) nil) rb2) st2))))
   | send_x : forall (c1 c2 : com) (sb1 sb2 : sb) (rb1 rb2 : rb) (st1 st2 : st)
                     (a : aexp) (x y z : id),
     dist_imp ((machine x c1 (state sb1 rb1 st1)),
              (machine y c2 (state (cons (a, x, z) sb2) rb2 st2))) 
-            ((machine x (RECEIVE ;; c1) 
-                (state sb1 (app (cons (a, z) nil) rb1) st1)),
+            ((machine x c1 (state sb1 (app (cons (a, z) nil) rb1) st1)),
             (machine y c2 (state sb2 rb2 st2))).
 
 Definition cdist_imp := multi dist_imp.
 
 Lemma proof_of_concept : forall x y n z,
   multi dist_imp ((machine x (SEND (ANum n) TO y CALLED z) empty_state),
-                 (machine y SKIP empty_state))
+                 (machine y (RECEIVE) empty_state))
                  ((machine x SKIP empty_state), 
-                 (machine y ((z ::= (ANum n) ;; SKIP)) empty_state)).
+                 (machine y (z ::= (ANum n)) empty_state)).
 Proof. 
   intros. eapply multi_step. apply imp_step_1. 
-    eapply CS_Send2. reflexivity.
+    eapply CS_Send4. reflexivity.
   eapply multi_step. apply send_y. fold empty_state. 
+  eapply multi_step. apply imp_step_2. apply CS_Rec4. fold empty_state. 
+  eapply multi_refl.   
+Qed.
+
+Lemma proof_of_concept' : forall x y z,
+  multi dist_imp ((machine x ((SEND (APlus (APlus (ANum 1) (ANum 1)) (ANum 1))
+                      TO y CALLED z) ;; RECEIVE) empty_state),
+                  (machine y (RECEIVE ;;
+                    SEND (APlus (APlus (ANum 1) (ANum 1)) (ANum 1)) TO x CALLED z)
+                    empty_state))
+                 ((machine x SKIP (state nil nil (t_update (t_empty 0) z 3))), 
+                  (machine y SKIP (state nil nil (t_update (t_empty 0) z 3)))).
+Proof.
+  intros. 
+  eapply multi_step. apply imp_step_2. apply CS_Rec1. 
+  eapply multi_step. apply imp_step_1. apply CS_Send1. apply AS_Plus1.
+    apply AS_Plus.
+  eapply multi_step. apply imp_step_1. apply CS_Send1. apply AS_Plus.
+  eapply multi_step. apply imp_step_1. eapply CS_Send2. reflexivity.
+  eapply multi_step. apply imp_step_2. apply CS_SeqSkip.
+  eapply multi_step. apply send_y. 
   eapply multi_step. apply imp_step_2. apply CS_Rec2.
-  fold empty_state. eapply multi_refl.   
+  eapply multi_step. apply imp_step_2. apply CS_SeqStep. apply CS_Ass.
+  eapply multi_step. apply imp_step_2. apply CS_SeqSkip.
+  eapply multi_step. apply imp_step_1. apply CS_SeqSkip.
+  eapply multi_step. apply imp_step_2. apply CS_Send3. apply AS_Plus1.
+    apply AS_Plus.
+  eapply multi_step. apply imp_step_2. apply CS_Send3. apply AS_Plus.
+  eapply multi_step. apply imp_step_2. eapply CS_Send4. reflexivity.
+  eapply multi_step. apply send_x.
+  eapply multi_step. apply imp_step_1. apply CS_Rec4.
+  eapply multi_step. apply imp_step_1. apply CS_Ass.
+  eapply multi_refl.
 Qed.
 
 End DistIMP.
